### 3.2-1

若 f(n) 和 g(n) 都是单调递增函数

=> 当 m < n 时, f(m) <= f(n), g(m) <= g(n)

=> 当 m < n 时, f(m) + g(m) <= f(n) + g(n) => f(n) + g(n) 单调递增

=> 当 m < n 时, f(g(m)) <= f(g(n)) => f(g(n)) 单调递增

=> 若 f(n) g(n) 非负, f(m)*g(m) <= f(n)*g(n) => f(n)*g(n)单调递增

### 3.2-2

证明 ![](http://latex.codecogs.com/gif.latex?a^{log_{b}c}=c^{log_{b}a})

![](http://latex.codecogs.com/gif.latex?a^{log_{b}c}=a^{\frac{log_{a}c}{log_{a}b}}=a^{log_{a}c\cdot%20log_{b}a}=c^{log_{b}a})

### 3.2-3

证明  ![](http://latex.codecogs.com/gif.latex?{lg(n!)}=\theta(nlgn))


### 3.2-4

